src/RIoT.Stubs.fst
@@ -3,7 +3,8 @@ module RIoT.Stubs
 open Common
 
 open LowStar.BufferOps
-open Lib.IntTypes
+//open Lib.IntTypes
+open FStar.Integers
 
 open Spec.Hash.Definitions
 open Hacl.Hash.Definitions
@@ -27,10 +28,140 @@ module M   = LowStar.Modifies
 module HS  = FStar.HyperStack
 module HST = FStar.HyperStack.ST
 
+/// <><><><><><><><<><><><><><><><><><><><><><><><><><><><><><><><>
+let rec memcpy
+  (#a)
+  (dst: B.buffer a)
+  (src: B.buffer a)
+  (len: I.uint_32)
+: HST.Stack unit
+  (requires fun h ->
+      B.live h dst
+    /\ B.live h src
+    /\ B.disjoint dst src
+    /\ len > 0ul
+    /\ len <= B.len src
+    /\ B.len src <= B.len dst)
+  (ensures  fun h0 _ h1 ->
+      M.modifies (M.loc_buffer dst) h0 h1
+/// TODO: /\ (B.get h1 dst (v len)) == (B.get h1 src (v len))
+/// TODO: /\ (S.slice (B.as_seq h1 dst) 0 (v len - 1)) `S.equal` (S.slice (B.as_seq h1 src) 0 (v len - 1))
+    )
+=
+  let cur = len - 1ul in
+  dst.(cur) <- src.(cur);
+  match cur with
+  | 0ul -> ()
+  | _   -> memcpy dst src cur
+
+let rec memset
+  (#a)
+  (dst: B.buffer a)
+  (v: a)
+  (len: I.uint_32)
+: HST.Stack unit
+  (requires fun h ->
+      B.live h dst
+    /\ len > 0ul
+    /\ len <= B.len dst)
+  (ensures  fun h0 _ h1 ->
+      M.modifies (M.loc_buffer dst) h0 h1
+/// TODO: /\ (S.slice (B.as_seq h1 dst) 0 (v len - 1)) `S.equal` (S.slice (B.as_seq h1 src) 0 (v len - 1))
+    )
+=
+  let cur = len - 1ul in
+  dst.(cur) <- v;
+  match cur with
+  | 0ul -> ()
+  | _   -> memset dst v cur
+
+let _BIGLEN : I.uint_32 = 0x09ul
+
+
+/// Size, in bytes, of a RIoT digest using the chosen hash algorithm.
+/// REF: #define RIOT_DIGEST_LENGTH      SHA256_DIGEST_LENGTH
+let _RIOT_DIGEST_LENGTH : I.uint_32 = hash_len SHA2_256
+
+/// Size, in bytes, of a RIoT HMAC.
+/// REF: #define RIOT_HMAC_LENGTH        RIOT_DIGEST_LENGTH
+let _RIOT_HMAC_LENGTH = _RIOT_DIGEST_LENGTH
+
+/// Size, in bytes, of internal keys used by the RIoT framework.
+/// NOTE:    This number of bytes is used for key derivation.
+/// REF: #define RIOT_KEY_LENGTH         RIOT_DIGEST_LENGTH
+let _RIOT_KEY_LENGTH = _RIOT_DIGEST_LENGTH
+
+/// Number of bits in internal symmetric keys used by the RIoT framework.
+/// NOTE:    This number of bits is used for key derivation. The symmetric
+///          algorithm implemenbted by the RIoT framework may use only a
+///          subset of these bytes for encryption.
+/// REF: #define RIOT_KEY_BITS           (RIOT_KEY_LENGTH * 8)
+let _RIOT_KEY_BITS = _RIOT_KEY_LENGTH
+
+/// Number of bytes in symmetric encryption keys used by the RIoT framework.
+/// This number also includes IV/Counter bytes.
+/// REF: #define RIOT_SYM_KEY_LENGTH             (16 + 16)
+let _RIOT_SYM_KEY_LENGT : I.uint_32 = 16ul + 16ul
+
+/// Size, in bytes, of encoded RIoT Key length
+/// REF: #define RIOT_ENCODED_BUFFER_MAX         (0x80)
+let _RIOT_ENCODED_BUFFER_MAX : I.uint_32 = 0x80ul
+
+/// Maximal number of bytes in a label/context passed to the RIoT KDF routine.
+/// REF: #define RIOT_MAX_KDF_CONTEXT_LENGTH     RIOT_DIGEST_LENGTH
+let _RIOT_MAX_KDF_CONTEXT_LENGTH : I.uint_32 = _RIOT_DIGEST_LENGTH
+
+/// Maximal number of bytes in a label/context passed to the RIoT KDF routine.
+/// REF: #define RIOT_MAX_KDF_LABEL_LENGTH       RIOT_DIGEST_LENGTH
+let _RIOT_MAX_KDF_CONTEXT_LABEL_LENGTH : I.uint_32 = _RIOT_DIGEST_LENGTH
+
+/// Maximal number of bytes in a RIOT_AIK certificate
+/// REF: #define RIOT_MAX_CERT_LENGTH        2048
+let _RIOT_MAX_CERT_LENGTH : I.uint_32 = 2048ul
+
+noeq
+type bigval_t = {
+     bigval : B.lbuffer HI.uint32 (v _BIGLEN)
+  }
+
+/// REF:
+/// typedef struct {
+///     bigval_t x;
+///     bigval_t y;
+///     uint32_t infinity;
+/// } affine_point_t;
+noeq
+type affine_point_t = {
+     x: bigval_t;
+     y: bigval_t;
+     infinity: B.pointer HI.uint32
+  }
+
+/// REF:
+/// typedef struct {
+///     bigval_t r;
+///     bigval_t s;
+/// } ECDSA_sig_t;
+noeq
+type ecdsa_sig_t = {
+     r: bigval_t;
+     s: bigval_t
+  }
+
+type ecc_signature  = ecdsa_sig_t
+type ecc_privatekey = bigval_t
+type ecc_publickey  = affine_point_t
+type ecc_secret     = affine_point_t
+
+type riot_ecc_signature  = ecc_signature
+type riot_ecc_publickey  = ecc_publickey
+type riot_ecc_privatekey = ecc_privatekey
+
+/// <><><><><><><><<><><><><><><><><><><><><><><><><><><><><><><><>
 assume val riotCrypt_Hash
-  (size: I.uint_32)
-  (data: B.lbuffer uint8 (v size))
-  (digest_alg: hash_alg)
+  (# size: I.uint_32)
+  (data: B.lbuffer HI.uint8 (v size))
+  (# digest_alg: hash_alg)
   (digest: hash_t digest_alg)
 : HST.Stack unit
   (requires fun h ->
@@ -43,10 +174,344 @@ assume val riotCrypt_Hash
 assume val riotCrypt_DeriveEccKey
   (public_key : riot_ecc_publickey)
   (private_key: riot_ecc_privatekey)
-  (digest_alg: hash_alg)
+  (#digest_alg: hash_alg)
   (digest: hash_t digest_alg)
-  (label_size: I.uint_32)
-  (label: B.lbuffer uint8 (I.v label_size))
+  (#label_size: I.uint_32)
+  (label: B.lbuffer HI.uint8 (I.v label_size))
+: HST.Stack unit
+  (requires fun h ->
+      B.live h public_key.x.bigval
+    /\ B.live h public_key.y.bigval
+    /\ B.live h public_key.infinity
+    /\ B.live h private_key.bigval
+    /\ B.live h digest
+    /\ B.live h label)
+  (ensures  fun h0 _ h1 -> True)
+
+/// Sets tbsData->SerialNumber to a quasi-random value derived from seedData
+/// REF: void RiotSetSerialNumber(RIOT_X509_TBS_DATA* tbsData, const uint8_t* seedData, size_t seedLen);
+assume val riotCrypt_SeedDRBG
+  //TODO: (tbsData: riot_X509_TBS_DATA)
+  (#seedLen: I.uint_32)
+  (seedData: B.lbuffer HI.uint8 (I.v seedLen))
+: HST.Stack unit
+  (requires fun h -> True)
+  (ensures  fun h0 _ h1 -> True)
+
+/// TODO: RIOT_STATUS
+
+///
+/// REF: RIOT_STATUS
+///      RiotCrypt_Sign(
+///          RIOT_ECC_SIGNATURE     *sig,        // OUT: Signature of data
+///          const void             *data,       // IN:  Data to sign
+///          size_t                  dataSize,   // IN:  Data size in bytes
+///          const RIOT_ECC_PRIVATE *key         // IN:  Signing key
+///      )
+assume val riotCrypt_Sign
+  (sig: riot_ecc_signature)
+  (#dataSize: I.uint_32)
+  (data: B.lbuffer HI.uint8 (v dataSize))
+  (key: riot_ecc_privatekey)
+: HST.Stack unit
+  (requires fun h -> True)
+  (ensures  fun h0 _ h1 -> True)
+///      {
+///          uint8_t digest[RIOT_DIGEST_LENGTH];
+///
+///          RiotCrypt_Hash(digest, sizeof(digest), data, dataSize);
+///
+///          return RIOT_DSASignDigest(digest, key, sig);
+///      }
+///
+
+///
+/// REF: RIOT_STATUS
+///      RiotCrypt_SignDigest(
+///          RIOT_ECC_SIGNATURE     *sig,            // OUT: Signature of digest
+///          const uint8_t          *digest,         // IN:  Digest to sign
+///          size_t                  digestSize,     // IN:  Size of the digest in bytes
+///          const RIOT_ECC_PRIVATE *key             // IN:  Signing key
+///      )
+///      {
+///          if (digestSize != RIOT_DIGEST_LENGTH) {
+///              return RIOT_INVALID_PARAMETER;
+///          }
+///
+///          return RIOT_DSASignDigest(digest, key, sig);
+///      }
+assume val riotCrypt_SignDigest
+  (sig: riot_ecc_signature)
+  (#digest_alg: hash_alg)
+  (digest: hash_t digest_alg)
+  (key: riot_ecc_publickey)
+: HST.Stack unit
+  (requires fun h -> True)
+  (ensures  fun h0 _ h1 -> True)
+
+/// REF: RIOT_STATUS
+///      RiotCrypt_Verify(
+///          const void                 *data,       // IN: Data to verify signature of
+///          size_t                      dataSize,   // IN: Size of data in bytes
+///          const RIOT_ECC_SIGNATURE   *sig,        // IN: Signature to verify
+///          const RIOT_ECC_PUBLIC      *key         // IN: ECC public key of signer
+///      )
+///      {
+///          uint8_t digest[RIOT_DIGEST_LENGTH];
+///
+///          RiotCrypt_Hash(digest, sizeof(digest), data, dataSize);
+///
+///          return RIOT_DSAVerifyDigest(digest, sig, key);
+///      }
+assume val riotCrypt_Verify
+  (#dataSize: I.uint_32)
+  (data: B.lbuffer HI.uint8 (v dataSize))
+  (sig: riot_ecc_signature)
+  (key: riot_ecc_publickey)
+: HST.Stack unit
+  (requires fun h -> True)
+  (ensures  fun h0 _ h1 -> True)
+
+/// REF: RIOT_STATUS
+///      RiotCrypt_VerifyDigest(
+///          const uint8_t              *digest,     // IN: Digest to verify signature of
+///          size_t                      digestSize, // IN: Size of the digest
+///          const RIOT_ECC_SIGNATURE   *sig,        // IN: Signature to verify
+///          const RIOT_ECC_PUBLIC      *key         // IN: ECC public key of signer
+///      )
+///      {
+///          if (digestSize != RIOT_DIGEST_LENGTH) {
+///              return RIOT_INVALID_PARAMETER;
+///          }
+///
+///          return RIOT_DSAVerifyDigest(digest, sig, key);
+///      }
+assume val riotCrypt_VerifyDigest
+  (#digest_alg: hash_alg)
+  (digest: hash_t digest_alg)
+  (sig: riot_ecc_signature)
+  (key: riot_ecc_publickey)
+: HST.Stack unit
+  (requires fun h -> True)
+  (ensures  fun h0 _ h1 -> True)
+
+///
+/// REF: RIOT_STATUS
+///      RiotCrypt_EccEncrypt(
+///          uint8_t                *result,         // OUT: Buffer to receive encrypted data
+///          size_t                  resultCapacity, // IN:  Capacity of the result buffer
+///          RIOT_ECC_PUBLIC        *ephKey,         // OUT: Ephemeral key to produce
+///          const void             *data,           // IN:  Data to encrypt
+///          size_t                  dataSize,       // IN:  Data size in bytes
+///          const RIOT_ECC_PUBLIC  *key             // IN:  Encryption key
+///      )
+assume val riotCrypt_EccEncrypt
+  (#resultCapacity: I.uint_32)
+  (result: B.lbuffer HI.uint8 (v resultCapacity))
+  (ephKey: riot_ecc_publickey)
+  (#dataSize: I.uint_32)
+  (data: B.lbuffer HI.uint8 (v dataSize))
+  (key: riot_ecc_publickey)
+: HST.Stack unit
+  (requires fun h -> True)
+  (ensures  fun h0 _ h1 -> True)
+///      {
+///          ecc_privatekey  ephPriv;
+///          ecc_secret      secret;
+///          uint8_t         exchKey[RIOT_KEY_LENGTH];
+///          RIOT_STATUS     status;
+///
+///          status = RIOT_GenerateDHKeyPair(ephKey, &ephPriv);
+///
+///          if (status != RIOT_SUCCESS) {
+///              return status;
+///          }
+///
+///          status = RIOT_GenerateShareSecret((RIOT_ECC_PUBLIC *)key, &ephPriv, &secret);
+///
+///          if (status != RIOT_SUCCESS) {
+///              return status;
+///          }
+///
+///          status = RiotCrypt_Kdf(exchKey, sizeof(exchKey),
+///                                 (uint8_t *)&secret, sizeof(secret),
+///                                 NULL, 0, (const uint8_t*)RIOT_LABEL_EXCHANGE,
+///                                 (sizeof(RIOT_LABEL_EXCHANGE) - 1),
+///                                 sizeof(exchKey));
+///
+///          if (status != RIOT_SUCCESS) {
+///              return status;
+///          }
+///
+///          status = RiotCrypt_SymEncryptDecrypt(result, resultCapacity,
+///                                               data, dataSize, exchKey);
+///          return status;
+///      }
+///
+
+
+///
+/// REF: RIOT_STATUS
+///      RiotCrypt_EccDecrypt(
+///          uint8_t                *result,         // OUT: Buffer to receive decrypted data
+///          size_t                  resultCapacity, // IN:  Capacity of the result buffer
+///          const void             *data,           // IN:  Data to decrypt
+///          size_t                  dataSize,       // IN:  Data size in bytes
+///          RIOT_ECC_PUBLIC        *ephKey,         // IN:  Ephemeral key to produce
+///          const RIOT_ECC_PRIVATE *key             // IN:  Decryption key
+///      )
+assume val riotCrypt_EccDecrypt
+  (#resultCapacity: I.uint_32)
+  (result: B.lbuffer HI.uint8 (v resultCapacity))
+  (ephKey: riot_ecc_publickey)
+  (#dataSize: I.uint_32)
+  (data: B.lbuffer HI.uint8 (v dataSize))
+  (key: riot_ecc_privatekey)
+: HST.Stack unit
+  (requires fun h -> True)
+  (ensures  fun h0 _ h1 -> True)
+///      {
+///          ecc_secret      secret;
+///          uint8_t         exchKey[RIOT_KEY_LENGTH];
+///          RIOT_STATUS     status;
+///
+///          status = RIOT_GenerateShareSecret(ephKey, (RIOT_ECC_PRIVATE *)key, &secret);
+///
+///          if (status != RIOT_SUCCESS) {
+///              return status;
+///          }
+///
+///          status = RiotCrypt_Kdf(exchKey, sizeof(exchKey),
+///                                 (uint8_t *)&secret, sizeof(secret),
+///                                 NULL, 0, (const uint8_t*)RIOT_LABEL_EXCHANGE,
+///                                 (sizeof(RIOT_LABEL_EXCHANGE) - 1),
+///                                 sizeof(exchKey));
+///
+///          if (status != RIOT_SUCCESS) {
+///              return status;
+///          }
+///
+///          status = RiotCrypt_SymEncryptDecrypt(result, resultCapacity,
+///                                               data, dataSize, exchKey);
+///          return status;
+///      }
+///      #endif
+///
+
+
+///
+/// REF: RIOT_STATUS
+///      RiotCrypt_SymEncryptDecrypt(
+///          void       *outData,                  // OUT: Output data
+///          size_t      outSize,                  // IN:  Size of output data
+///          const void *inData,                   // IN:  Input data
+///          size_t      inSize,                   // IN:  Size of input data
+///          uint8_t     key[RIOT_SYM_KEY_LENGTH]  // IN/OUT: Symmetric key & IV
+///      )
+assume val riotCrypt_SymEncryptDecrypt
+  (#outSize: I.uint_32)
+  (outData: B.lbuffer HI.uint32 (I.v outSize))
+  (#inSize: I.uint_32)
+  (inData: B.lbuffer HI.uint32 (I.v inSize))
+  (key: B.lbuffer HI.uint8 _RIOT_SYM_KEY_LENGT)
+: HST.Stack unit
+  (requires fun h -> True)
+  (ensures  fun h0 _ h1 -> True)
+///      {
+///          uint8_t             *iv = key + 16;
+///          aes128EncryptKey_t  aesKey;
+///
+///          if (outSize < inSize) {
+///              return RIOT_INVALID_PARAMETER;
+///          }
+///
+///          RIOT_AES128_Enable(key, &aesKey);
+///          RIOT_AES_CTR_128((const aes128EncryptKey_t*) &aesKey, inData, outData, (uint32_t)inSize, iv);
+///          RIOT_AES128_Disable(&aesKey);
+///
+///          return RIOT_SUCCESS;
+///      }
+
+assume val riotCrypt_Sign
+  (u:unit)
+: HST.Stack unit
+  (requires fun h -> True)
+  (ensures  fun h0 _ h1 -> True)
+
+assume val riotCrypt_Verify
+  (u:unit)
+: HST.Stack unit
+  (requires fun h -> True)
+  (ensures  fun h0 _ h1 -> True)
+
+assume val riotCrypt_ExportEccPub
+  (u:unit)
+: HST.Stack unit
+  (requires fun h -> True)
+  (ensures  fun h0 _ h1 -> True)
+
+assume val riotSetSerialNumber
+  (u:unit)
+: HST.Stack unit
+  (requires fun h -> True)
+  (ensures  fun h0 _ h1 -> True)
+
+assume val derInitContext
+  (u:unit)
+: HST.Stack unit
+  (requires fun h -> True)
+  (ensures  fun h0 _ h1 -> True)
+
+assume val x509GetAliasCertTBS
+  (u:unit)
+: HST.Stack unit
+  (requires fun h -> True)
+  (ensures  fun h0 _ h1 -> True)
+
+assume val x509GetRootCertTBS
+  (u:unit)
+: HST.Stack unit
+  (requires fun h -> True)
+  (ensures  fun h0 _ h1 -> True)
+
+assume val x509MakeRootCert
+  (u:unit)
+: HST.Stack unit
+  (requires fun h -> True)
+  (ensures  fun h0 _ h1 -> True)
+
+assume val x509MakeDeviceCert
+  (u:unit)
+: HST.Stack unit
+  (requires fun h -> True)
+  (ensures  fun h0 _ h1 -> True)
+
+assume val x509GetDERCsrTbs
+  (u:unit)
+: HST.Stack unit
+  (requires fun h -> True)
+  (ensures  fun h0 _ h1 -> True)
+
+assume val x509GetDERCsr
+  (u:unit)
+: HST.Stack unit
+  (requires fun h -> True)
+  (ensures  fun h0 _ h1 -> True)
+
+assume val x509MakeAliasCert
+  (u:unit)
+: HST.Stack unit
+  (requires fun h -> True)
+  (ensures  fun h0 _ h1 -> True)
+
+assume val der_to_pem
+  (u:unit)
+: HST.Stack unit
+  (requires fun h -> True)
+  (ensures  fun h0 _ h1 -> True)
+
+assume val firmwareEntry
+  (u:unit)
 : HST.Stack unit
   (requires fun h -> True)
   (ensures  fun h0 _ h1 -> True)
